Veir/Passes/LLVMToGMIR.lean
@@ -1,46 +1,68 @@
 module
 
 public import Veir.Pass
-public import Veir.PatternRewriter.Basic
 import Veir.Passes.Matching
-
-/-!
-  # LLVMToGMIR pass
-
-  Lowers every (not yet) operation of the `llvm` dialect into the `gMIR` dialect.
-  This corresponds to LLVM's `IRTranslator` in GlobalISel (`llvm/CodeGen/GlobalISel/IRTranslator.h`).
-
-  Currently, mostly copied code from ArithToLLVM.
--/
+import Veir.PatternRewriter.Puddle.Builders
+import Veir.PatternRewriter.Puddle.Execution
 
 namespace Veir
 
-/-! ## Generic 1:1 lowering -/
+/-!
+  This file replicates LLVM's GlobalISel IRTranslator pass.
+  This pass is responsible for translating LLVM IR into gMIR.
 
+  The properties of all LLVM-IR instruction are carried over into gMIR
+  (see upstreams `MachineInstr::copyFlagsFromInstruction`).
+-/
+
+/-! # Lowering Patterns -/
+
+/--
+  gMIR 1:1 lowerings with Puddle for binary integer operations.
+
+  This mirrors ArithToLLVM's lower1to1.
+-/
 def lower1to1 (lOp : Llvm) (gOp : GMIR)
-    (convert : propertiesOf (OpCode.llvm lOp) → propertiesOf (OpCode.gmir gOp)) (numOperands : Nat)
-    (rewriter : PatternRewriter OpCode) (op : OperationPtr)
-    (_opInBounds : op.InBounds rewriter.ctx.raw) : Option (PatternRewriter OpCode) := do
-  let some (operands, props) := matchOp op rewriter.ctx.raw lOp numOperands
-    | return rewriter
-  let ip := InsertPoint.before op
-  let (rewriter, newOp) ← rewriter.createOp! (.gmir gOp)
-    (op.getResultTypes! rewriter.ctx.raw) operands #[] #[] (convert props) (some ip)
-  let rewriter := rewriter.replaceValue! (op.getResult 0) (newOp.getResult 0)
-  return rewriter.eraseOp! op
+    (h : propertiesOf (OpCode.llvm lOp) = propertiesOf (OpCode.gmir gOp) := by rfl) :
+    Puddle.Pattern OpCode :=
+  let info := gOp.genericOpInfo
+  Puddle.Pattern.Builder
+    (do
+      let root ← Puddle.MatchProg.root (.llvm lOp) #[] #[]
+      let operands ← Puddle.MatchProg.operands root.op info.inOperandList.size
+      let returnTypes ← Puddle.MatchProg.resultTypes root.op info.outOperandList.size
+      return (returnTypes, operands, root))
+    (fun (returnTypes, operands, root) => do
+      let props ← Puddle.CreateProg.applyNative root.properties
+                    (fun p => some (cast h p))
+      let newOp ← Puddle.CreateProg.operation (.gmir gOp) operands returnTypes props
+      return newOp)
+    (fun newOp => newOp)
 
-/-! ### The 1:1 patterns -/
+def g_add_pattern := lower1to1 .add .g_add
 
-def lowerAdd  := lower1to1 .add  .g_add  (fun p => p) 2
-def lowerSub  := lower1to1 .sub  .g_sub  (fun p => p) 2
-def lowerIcmp := lower1to1 .icmp .g_icmp (fun p => p) 2
+def g_sub_pattern := lower1to1 .sub .g_sub
 
-/-! ## Pass implementation -/
+def g_icmp_pattern := lower1to1 .icmp  .g_icmp
+
+def g_add (rewriter : PatternRewriter OpCode) (op : OperationPtr)
+    (opInBounds : op.InBounds rewriter.ctx.raw) : Option (PatternRewriter OpCode) :=
+  RewritePattern.fromLocalRewrite g_add_pattern.compile rewriter op opInBounds
+
+def g_sub (rewriter : PatternRewriter OpCode) (op : OperationPtr)
+    (opInBounds : op.InBounds rewriter.ctx.raw) : Option (PatternRewriter OpCode) :=
+  RewritePattern.fromLocalRewrite g_sub_pattern.compile rewriter op opInBounds
+
+def g_icmp (rewriter : PatternRewriter OpCode) (op : OperationPtr)
+    (opInBounds : op.InBounds rewriter.ctx.raw) : Option (PatternRewriter OpCode) :=
+  RewritePattern.fromLocalRewrite g_icmp_pattern.compile rewriter op opInBounds
+
+/-! # Pass implementation -/
 
 def LLVMToGMIRPass.impl (ctx : WfIRContext OpCode) (op : OperationPtr)
     (_ : op.InBounds ctx.raw) : ExceptT String IO (WfIRContext OpCode) := do
   let pattern := RewritePattern.GreedyRewritePattern #[
-    lowerAdd, lowerSub, lowerIcmp
+    g_add, g_sub, g_icmp
   ]
   match RewritePattern.applyInContext pattern ctx with
   | none => throw "Error while applying llvm-to-gmir translation"
